Just as in standard algebra, various rules can be applied to simplify Boolean algebra expressions. These simplifications help in making logical expressions clearer and more efficient.

---
### **De Morgan’s Laws**
De Morgan’s laws describe how to negate expressions involving conjunction (AND) and disjunction (OR). The laws state:

1. **Negation of Conjunction**:
    ¬(A∧B)≡¬A∨¬B\neg (A \land B) \equiv \neg A \lor \neg B¬(A∧B)≡¬A∨¬B
2. **Negation of Disjunction**:
    ¬(A∨B)≡¬A∧¬B\neg (A \lor B) \equiv \neg A \land \neg B¬(A∨B)≡¬A∧¬B

These laws are useful for transforming complex expressions, especially when negation applies to the entire expression.

---
### **Distribution**
Distribution applies to conjunction and disjunction, allowing you to distribute one operation over another.
1. **Conjunction over Disjunction**:
    A∧(B∨C)≡(A∧B)∨(A∧C)A \land (B \lor C) \equiv (A \land B) \lor (A \land C)A∧(B∨C)≡(A∧B)∨(A∧C)
2. **Disjunction over Conjunction**:
    A∨(B∧C)≡(A∨B)∧(A∨C)A \lor (B \land C) \equiv (A \lor B) \land (A \lor C)A∨(B∧C)≡(A∨B)∧(A∨C)

Distribution can also occur over the same operator, which is important for simplifying expressions further.

---
### **Association**
The associative laws allow for the addition or removal of parentheses in expressions, which can help in rearranging terms without changing the result.
- **For conjunction**:
    A∧(B∧C)≡(A∧B)∧C≡A∧B∧CA \land (B \land C) \equiv (A \land B) \land C \equiv A \land B \land CA∧(B∧C)≡(A∧B)∧C≡A∧B∧C
- **For disjunction**:
    A∨(B∨C)≡(A∨B)∨C≡A∨B∨CA \lor (B \lor C) \equiv (A \lor B) \lor C \equiv A \lor B \lor CA∨(B∨C)≡(A∨B)∨C≡A∨B∨C

---
### **Commutation**
The commutative laws demonstrate that the order of the literals around an operator does not affect the outcome.
- **For conjunction**:
    A∧B≡B∧AA \land B \equiv B \land AA∧B≡B∧A
- **For disjunction**:
    A∨B≡B∨AA \lor B \equiv B \lor AA∨B≡B∨A

---
### **Double Negation**
The double negation law states that negating a literal twice returns the original literal:

¬(¬A)≡A\neg (\neg A) \equiv A¬(¬A)≡A

This principle simplifies expressions by allowing the removal of redundant negations.